DeepAndShallowEmbeddings: adding failure

DeeperWithFailInterp.ml
@@ -1,0 +1,29 @@
+let rec i2n n =
+  match n with
+  | 0 -> O
+  | _ -> S (i2n (n - 1))
+
+let interp c =
+  let h : (nat, nat) Hashtbl.t = Hashtbl.create 0 in
+  Hashtbl.add h (i2n 0) (i2n 2);
+  Hashtbl.add h (i2n 1) (i2n 1);
+  Hashtbl.add h (i2n 2) (i2n 8);
+  Hashtbl.add h (i2n 3) (i2n 6);
+
+  let rec interp' (c : 'a cmd) : 'a =
+    match c with
+    | Return v -> v
+    | Bind (c1, c2) -> interp' (c2 (interp' c1))
+    | Read a ->
+      Obj.magic (try
+                   Hashtbl.find h a
+        with Not_found -> O)
+    | Write (a, v) -> Obj.magic (Hashtbl.replace h a v)
+    | Loop (i, b) ->
+      begin match Obj.magic (interp' (Obj.magic (b i))) with
+      | Done r -> r
+      | Again r -> interp' (Loop (r, b))
+      end
+    | Fail -> failwith "Fail"
+
+  in h, interp' c
