DeepAndShallowEmbeddings.v
@@ -655,3 +655,339 @@ Module Deeper.
 
   Extraction "Deeper.ml" index_of.
 End Deeper.
+
+
+(** * Adding the possibility of program failure *)
+
+Module DeeperWithFail.
+  Inductive loop_outcome acc :=
+  | Done (a : acc)
+  | Again (a : acc).
+
+  Inductive cmd : Set -> Type :=
+  | Return {result : Set} (r : result) : cmd result
+  | Bind {result result'} (c1 : cmd result') (c2 : result' -> cmd result) : cmd result
+  | Read (a : nat) : cmd nat
+  | Write (a v : nat) : cmd unit
+  | Loop {acc : Set} (init : acc) (body : acc -> cmd (loop_outcome acc)) : cmd acc
+  | Fail {result} : cmd result.
+
+  Notation "x <- c1 ; c2" := (Bind c1 (fun x => c2)) (right associativity, at level 80).
+  Notation "'for' x := i 'loop' c1 'done'" := (Loop i (fun x => c1)) (right associativity, at level 80).
+
+  Definition forever : cmd nat :=
+    _ <- Write 0 1;
+    for i := 1 loop
+      h_i <- Read i;
+      acc <- Read 0;
+      match acc with
+      | 0 => Fail
+      | _ =>
+        _ <- Write 0 (acc + h_i);
+        Return (Again (i + 1))
+      end
+    done.
+
+  Inductive stepResult (result : Set) :=
+  | Answer (r : result)
+  | Stepped (h : heap) (c : cmd result)
+  | Failed.
+
+  Implicit Arguments Failed [result].
+
+  Fixpoint step {result} (c : cmd result) (h : heap) : stepResult result :=
+    match c with
+    | Return r => Answer r
+    | Bind c1 c2 =>
+      match step c1 h with
+      | Answer r => Stepped h (c2 r)
+      | Stepped h' c1' => Stepped h' (Bind c1' c2)
+      | Failed => Failed
+      end
+    | Read a => Answer (h $! a)
+    | Write a v => Stepped (h $+ (a, v)) (Return tt)
+    | Loop init body =>
+      Stepped h (r <- body init;
+                 match r with
+                 | Done r' => Return r'
+                 | Again r' => Loop r' body
+                 end)
+    | Fail => Failed
+    end.
+
+  Fixpoint multiStep {result} (c : cmd result) (h : heap) (n : nat) : stepResult result :=
+    match n with
+    | O => Stepped h c
+    | S n' => match step c h with
+              | Answer r => Answer r
+              | Stepped h' c' => multiStep c' h' n'
+              | Failed => Failed
+              end
+    end.
+
+  Inductive hoare_triple : assertion -> forall {result}, cmd result -> (result -> assertion) -> Prop :=
+  | HtReturn : forall P {result : Set} (v : result),
+      hoare_triple P (Return v) (fun r h => P h /\ r = v)
+  | HtBind : forall P {result' result} (c1 : cmd result') (c2 : result' -> cmd result) Q R,
+      hoare_triple P c1 Q
+      -> (forall r, hoare_triple (Q r) (c2 r) R)
+      -> hoare_triple P (Bind c1 c2) R
+  | HtRead : forall P a,
+      hoare_triple P (Read a) (fun r h => P h /\ r = h $! a)
+  | HtWrite : forall P a v,
+      hoare_triple P (Write a v) (fun _ h => exists h', P h' /\ h = h' $+ (a, v))
+  | HtConsequence : forall {result} (c : cmd result) P Q (P' : assertion) (Q' : _ -> assertion),
+      hoare_triple P c Q
+      -> (forall h, P' h -> P h)
+      -> (forall r h, Q r h -> Q' r h)
+      -> hoare_triple P' c Q'
+
+  | HtLoop : forall {acc : Set} (init : acc) (body : acc -> cmd (loop_outcome acc)) I,
+      (forall acc, hoare_triple (I (Again acc)) (body acc) I)
+      -> hoare_triple (I (Again init)) (Loop init body) (fun r h => I (Done r) h)
+
+  | HtFail : forall {result},
+      hoare_triple (fun _ => False) (Fail (result := result)) (fun _ _ => False).
+
+  Notation "{{ h ~> P }} c {{ r & h' ~> Q }}" :=
+    (hoare_triple (fun h => P) c (fun r h' => Q)) (at level 90, c at next level).
+
+  Lemma HtStrengthen : forall {result} (c : cmd result) P Q (Q' : _ -> assertion),
+      hoare_triple P c Q
+      -> (forall r h, Q r h -> Q' r h)
+      -> hoare_triple P c Q'.
+  Proof.
+    simplify.
+    eapply HtConsequence; eauto.
+  Qed.
+
+  Lemma HtWeaken : forall {result} (c : cmd result) P Q (P' : assertion),
+      hoare_triple P c Q
+      -> (forall h, P' h -> P h)
+      -> hoare_triple P' c Q.
+  Proof.
+    simplify.
+    eapply HtConsequence; eauto.
+  Qed.
+
+  Theorem forever_ok :
+    {{ _ ~> True }}
+      forever
+    {{ _&_ ~> False }}.
+  Proof.
+    unfold forever.
+    econstructor.
+    econstructor.
+    simplify.
+    eapply HtConsequence.
+    apply HtLoop with (I := fun r h => h $! 0 > 0 /\ match r with
+                                                     | Done _ => False
+                                                     | _ => True
+                                                     end); simplify.
+
+    econstructor.
+    econstructor.
+    simplify.
+    econstructor.
+    econstructor.
+    simplify.
+    cases r1.
+    eapply HtConsequence.
+    apply HtFail.
+    simplify.
+    linear_arithmetic.
+    simplify.
+    linear_arithmetic.
+    econstructor.
+    econstructor.
+    simplify.
+    eapply HtStrengthen.
+    econstructor.
+    simplify.
+    propositional; subst.
+    invert H0; propositional; subst.
+    simplify.
+    linear_arithmetic.
+    invert H0; propositional; subst.
+    simplify.
+    invert H; propositional; subst.
+    simplify.
+    linear_arithmetic.
+    simplify.
+    propositional.
+  Qed.
+
+  Definition trsys_of {result} (c : cmd result) (h : heap) := {|
+    Initial := {(c, h)};
+    Step := fun p1 p2 => step (fst p1) (snd p1) = Stepped (snd p2) (fst p2)
+  |}.
+
+  Lemma invert_Return : forall {result : Set} (r : result) P Q,
+    hoare_triple P (Return r) Q
+    -> forall h, P h -> Q r h.
+  Proof.
+    induct 1; propositional; eauto.
+  Qed.
+
+  Lemma invert_Bind : forall {result' result} (c1 : cmd result') (c2 : result' -> cmd result) P Q,
+    hoare_triple P (Bind c1 c2) Q
+    -> exists R, hoare_triple P c1 R
+                 /\ forall r, hoare_triple (R r) (c2 r) Q.
+  Proof.
+    induct 1; propositional; eauto.
+
+    invert IHhoare_triple; propositional.
+    eexists; propositional.
+    eapply HtWeaken.
+    eassumption.
+    auto.
+    eapply HtStrengthen.
+    apply H4.
+    auto.
+  Qed.
+
+  Lemma unit_not_nat : unit = nat -> False.
+  Proof.
+    simplify.
+    assert (exists x : unit, forall y : unit, x = y).
+    exists tt; simplify.
+    cases y; reflexivity.
+    rewrite H in H0.
+    invert H0.
+    specialize (H1 (S x)).
+    linear_arithmetic.
+  Qed.
+
+  Lemma invert_Read : forall a P Q,
+    hoare_triple P (Read a) Q
+    -> forall h, P h -> Q (h $! a) h.
+  Proof.
+    induct 1; propositional; eauto.
+    apply unit_not_nat in x0.
+    propositional.
+  Qed.
+
+  Lemma invert_Write : forall a v P Q,
+    hoare_triple P (Write a v) Q
+    -> forall h, P h -> Q tt (h $+ (a, v)).
+  Proof.
+    induct 1; propositional; eauto.
+    symmetry in x0.
+    apply unit_not_nat in x0.
+    propositional.
+  Qed.
+
+  Lemma invert_Loop : forall {acc : Set} (init : acc) (body : acc -> cmd (loop_outcome acc)) P Q,
+      hoare_triple P (Loop init body) Q
+      -> exists I, (forall acc, hoare_triple (I (Again acc)) (body acc) I)
+                   /\ (forall h, P h -> I (Again init) h)
+                   /\ (forall r h, I (Done r) h -> Q r h).
+  Proof.
+    induct 1; propositional; eauto.
+
+    invert IHhoare_triple; propositional.
+    exists x; propositional; eauto.
+  Qed.
+
+  Lemma invert_Fail : forall result P Q,
+    hoare_triple P (Fail (result := result)) Q
+    -> forall h, P h -> False.
+  Proof.
+    induct 1; propositional; eauto.
+  Qed.
+
+  Lemma step_sound : forall {result} (c : cmd result) h Q,
+      hoare_triple (fun h' => h' = h) c Q
+      -> match step c h with
+         | Answer r => Q r h
+         | Stepped h' c' => hoare_triple (fun h'' => h'' = h') c' Q
+         | Failed => False
+         end.
+  Proof.
+    induct c; simplify; propositional.
+
+    eapply invert_Return.
+    eauto.
+    simplify; auto.
+
+    apply invert_Bind in H0.
+    invert H0; propositional.
+    apply IHc in H0.
+    cases (step c h); auto.
+    econstructor.
+    apply H2.
+    equality.
+    auto.
+    econstructor; eauto.
+
+    eapply invert_Read; eauto.
+    simplify; auto.
+
+    eapply HtStrengthen.
+    econstructor.
+    simplify; propositional; subst.
+    eapply invert_Write; eauto.
+    simplify; auto.
+
+    apply invert_Loop in H0.
+    invert H0; propositional.
+    econstructor.
+    eapply HtWeaken.
+    apply H0.
+    equality.
+    simplify.
+    cases r.
+    eapply HtStrengthen.
+    econstructor.
+    simplify.
+    propositional; subst; eauto.
+    eapply HtStrengthen.
+    eapply HtLoop.
+    auto.
+    simplify.
+    eauto.
+
+    eapply invert_Fail; eauto.
+    simplify; eauto.
+  Qed.
+
+  Lemma hoare_triple_sound' : forall P {result} (c : cmd result) Q,
+      hoare_triple P c Q
+      -> forall h, P h
+                   -> invariantFor (trsys_of c h)
+                                   (fun p => hoare_triple (fun h => h = snd p)
+                                                          (fst p)
+                                                          Q).
+  Proof.
+    simplify.
+
+    apply invariant_induction; simplify.
+
+    propositional; subst; simplify.
+    eapply HtConsequence.
+    eassumption.
+    equality.
+    auto.
+
+    eapply step_sound in H1.
+    rewrite H2 in H1.
+    auto.
+  Qed.
+
+  Theorem hoare_triple_sound : forall P {result} (c : cmd result) Q,
+      hoare_triple P c Q
+      -> forall h, P h
+                   -> invariantFor (trsys_of c h)
+                                   (fun p => step (fst p) (snd p) <> Failed).
+  Proof.
+    simplify.
+
+    eapply invariant_weaken.
+    eapply hoare_triple_sound'; eauto.
+    simplify.
+    eapply step_sound in H1.
+    cases (step (fst s) (snd s)); equality.
+  Qed.
+
+  Extraction "DeeperWithFail.ml" forever.
+End DeeperWithFail.
